minimize PR footprint

tests/lean/run/grind_pp_attr.lean
@@ -1,11 +1,14 @@
 import Lean.Elab.Command
 
-/-!
-# Pretty-printing of the `grind` attribute
--/
+open Lean Elab Command
 
-elab "#pp " c:command : command => do
-  Lean.logInfo c
+def test (stx : Syntax) : CommandElabM Unit := do
+  let fmt : Option Format := ←
+        liftCoreM <| PrettyPrinter.ppCategory `command stx
+  if let some fmt := fmt then
+  let st := fmt.pretty
+  dbg_trace st
+
 
 /--
 info: @[grind =]
@@ -13,7 +16,7 @@ example :=
   0
 -/
 #guard_msgs in
-#pp @[grind =] example := 0
+run_cmd test (← `(@[grind =] example := 0))
 
 /--
 info: @[grind _=_]
@@ -21,7 +24,7 @@ example :=
   0
 -/
 #guard_msgs in
-#pp  @[grind _=_] example := 0
+run_cmd test (← `(@[grind _=_] example := 0))
 
 /--
 info: @[grind =_]
@@ -29,7 +32,7 @@ example :=
   0
 -/
 #guard_msgs in
-#pp @[grind =_] example := 0
+run_cmd test (← `(@[grind =_] example := 0))
 
 /--
 info: @[grind →]
@@ -37,7 +40,7 @@ example :=
   0
 -/
 #guard_msgs in
-#pp @[grind →] example := 0
+run_cmd test (← `(@[grind →] example := 0))
 
 /--
 info: @[grind ←]
@@ -45,7 +48,7 @@ example :=
   0
 -/
 #guard_msgs in
-#pp @[grind ←] example := 0
+run_cmd test (← `(@[grind ←] example := 0))
 
 /--
 info: @[grind ←=]
@@ -53,7 +56,7 @@ example :=
   0
 -/
 #guard_msgs in
-#pp @[grind ←=] example := 0
+run_cmd test (← `(@[grind ←=] example := 0))
 
 /--
 info: @[grind]
@@ -61,7 +64,7 @@ example :=
   0
 -/
 #guard_msgs in
-#pp @[grind] example := 0
+run_cmd test (← `(@[grind] example := 0))
 
 /--
 info: @[grind ← gen]
@@ -69,12 +72,8 @@ example :=
   0
 -/
 #guard_msgs in
-#pp @[grind ← gen] example := 0
+run_cmd test (← `(@[grind ← gen] example := 0))
 
 /-- info: example := by grind [a] on_failure 3 -/
 #guard_msgs in
-#pp example := by grind [a] on_failure 3
-
-/-- info: example := by grind [← a] on_failure 3 -/
-#guard_msgs in
-#pp example := by grind [← a] on_failure 3
+run_cmd test (← `(example := by grind [a] on_failure 3))
